refinement for memory read and update asid

Case_Study/Mode_Switch.thy
@@ -25,6 +25,10 @@ lemma f_incon_set_upd[simp]:
   "f (incon_set_update upd s) = f s"
   by (rule heap_eq) simp
 
+lemma f_ptable_snapshot_set_upd[simp]:
+  "f (ptable_snapshot_update upd s) = f s"
+  by (rule heap_eq) simp
+
 lemma f_asid_upd[simp]:
   "f (p_state.asid_update upd s) = f s"
   by (rule heap_eq) simp
@@ -121,19 +125,98 @@ where
   "\<I>\<C> s \<equiv>  {vp. (asid s, Addr vp) \<in> incon_set s}" 
 
 
+
+(* have new conditions for tlb_snapshot *)
+
+
+(* it is a lookup type, which means that we have to assume that from tlb_rel that, 
+  in the start, the tlb_snanpshot will be miss, no incon and no hit, so lets assume that  *)
+
+
+definition
+  "snap_not_incon S s \<equiv> \<forall>a\<in>(ran (root_map s) - S). \<forall>v. ptable_snapshot s a v \<noteq> Incon"
+
+(* we can only specify the subset condition *)
+
+definition
+  "snap_miss_or_consistent_hit snp a mem rt \<equiv> \<forall>v. snp a v = Miss \<or> snp a v = Hit (pt_walk a mem rt v)"
+
+
+(* context switch code from sel4
+     /*
+     * On ARMv7, speculative refills that complete between switching
+     * ASID and PD can cause TLB entries to be Tagged with the wrong
+     * ASID. The correct method to avoid this problem is to
+     * either cycle the context switch through a reserved ASID or
+     * through a page directory that has only global mappings.
+     * The reserved Page directory method has shown to perform better
+     * than the reserved ASID method.
+     *
+     * We do not call setCurrentPD here as we want to perform a
+     * minimal number of DSB and ISBs and the second PD switch we
+     * do does not need a DSB
+     */
+    dsb();
+    writeTTBR0(addrFromPPtr(armKSGlobalPD));
+    isb();
+    setHardwareASID(hw_asid);
+    writeTTBR0(addrFromPPtr(cap_pd));
+    isb();
+
+*)
+
+definition "snp_incon_constraint S s \<equiv> {(a,v). a\<in>(ran (root_map s) - S) \<and> ptable_snapshot s a v = Incon }  \<subseteq>  incon_set s"
+
+(* we assume that the flush has happened after write to the page table *)
+
+lemma
+  "\<lbrakk>snp_incon_constraint S s ; asids_consistent {} s \<rbrakk>  \<Longrightarrow> snap_not_incon S s"
+  apply (clarsimp simp: snp_incon_constraint_def ptable_snapshot_def asids_consistent_def ran_def snap_not_incon_def)
+  by blast
+
+
 lemma new_context_switch:
-  "\<Turnstile> \<lbrace> \<lambda>s. mmu_layout s \<and> asids_consistent {} s \<and> mode s = Kernel \<and>
+  "\<Turnstile> \<lbrace> \<lambda>s. mmu_layout s \<and> asids_consistent {} s \<and> mode s = Kernel \<and> snp_incon_constraint {} s \<and>  
+           snap_miss_or_consistent_hit (ptable_snapshot s) a (heap s) (Addr r) \<and> 
             0 \<notin> ran (root_map s) \<and> root_map s (Addr r) = Some a \<and> Addr r \<in> root_log s\<rbrace>
             UpdateASID 0 ;; UpdateTTBR0 (Const r) ;; UpdateASID a ;; SetMode User
       \<lbrace>\<lambda>s. mmu_layout s \<and> \<I>\<C> s = {} \<and> mode s = User \<and> asids_consistent {} s \<rbrace>"
+  (* may not be true in its current form *)
+
+(* what should we have for the paper? same concept as asid 0?*)
+
   apply vcgm
-  apply (clarsimp simp: mmu_layout_def)  
-  apply (clarsimp simp: \<I>\<C>_def asids_consistentD)
-  apply (rule conjI, clarsimp)
+  apply (rule conjI)
+   apply (clarsimp simp: mmu_layout_def)  
+  apply (rule conjI)
+   apply (clarsimp simp: \<I>\<C>_def asids_consistentD)
+   apply (rule conjI, clarsimp)
+    apply (clarsimp simp: incon_load_def  snapshot_update_current'_def  snapshot_update_current_def ran_def)
+   apply (rule conjI)
+    apply (clarsimp simp: asids_consistent_def pde_comp_def Let_def times_Int_times Int_Un_distrib ran_def)
+   apply clarsimp
+   apply (simp only: incon_load_def  snapshot_update_current'_def  snapshot_update_current_def  snapshot_update_new'_def snapshot_update_new_def)
+  apply safe [1]
+
+
+
+
+(*
+   apply (clarsimp simp: incon_load_def  snapshot_update_current'_def  snapshot_update_current_def  snapshot_update_new'_def snapshot_update_new_def)
+   apply safe [1]
+     apply (clarsimp simp: ran_def)
+    apply (clarsimp simp: asids_consistent_def pde_comp_def Let_def times_Int_times Int_Un_distrib ran_def)
+  apply auto [1]
+ apply (clarsimp simp: ran_def)
    apply (erule ptable_comp_asid)
    apply (clarsimp simp: ran_def)
-  apply (simp add: asids_consistent_def pde_comp_def Let_def times_Int_times Int_Un_distrib)
-  done
+  apply (clarsimp simp: asids_consistent_def pde_comp_def Let_def times_Int_times Int_Un_distrib)
+
+*)
+
+
+
+  sorry
 
 end
 
