MMU_ARMv7_Refinement_No_Fault/ARMv7_TLB_Ref_Func.thy
@@ -1,0 +1,385 @@
+theory ARMv7_TLB_Ref_Func
+
+imports  MMU_ARM.ARM_Monadic
+
+begin               
+
+
+
+
+record tlb_state = state + 
+           tlb_set :: "tlb_entry set "
+
+
+record tlb_det_state = state + 
+           tlb_det_set :: "tlb_entry set"
+
+
+record tlb_sat_no_flt_state = state + 
+           tlb_sat_no_flt_set :: "tlb_entry set"
+
+
+record tlb_incon_set' =
+  incon_set    :: "(asid \<times> vaddr) set"
+  tlb_snapshot :: "asid \<Rightarrow> vaddr \<Rightarrow> lookup_type"
+
+
+record tlb_incon_state' = state + 
+           tlb_incon_set' :: tlb_incon_set'
+
+
+
+definition 
+  typ_tlb :: "'a tlb_state_scheme \<Rightarrow> tlb_entry set state_scheme"
+where
+  "typ_tlb s =  state.extend (state.truncate s) (tlb_set s)"
+
+
+definition 
+  typ_det_tlb :: "'a tlb_det_state_scheme \<Rightarrow> tlb_entry set state_scheme"
+where
+  "typ_det_tlb s =  state.extend (state.truncate s) (tlb_det_set s)"
+
+
+
+definition 
+  typ_sat_no_flt_tlb :: "'a tlb_sat_no_flt_state_scheme \<Rightarrow> tlb_entry set state_scheme"
+where
+  "typ_sat_no_flt_tlb s =  state.extend (state.truncate s) (tlb_sat_no_flt_set s)"
+
+
+
+definition 
+  typ_incon' :: "'a tlb_incon_state'_scheme \<Rightarrow> tlb_incon_set' state_scheme"
+where
+  "typ_incon' s =  state.extend (state.truncate s) (tlb_incon_set' s)"
+
+
+lemma tlb_more [simp]:
+  "state.more (typ_tlb s) = tlb_set s"
+  by (clarsimp simp: typ_tlb_def state.defs)
+
+
+lemma tlb_det_more [simp]:
+  "state.more (typ_det_tlb s) = tlb_det_set s"
+  by (clarsimp simp: typ_det_tlb_def state.defs)
+
+
+lemma tlb_sat_no_flt_more [simp]:
+  "state.more (typ_sat_no_flt_tlb s) = tlb_sat_no_flt_set s"
+  by (clarsimp simp: typ_sat_no_flt_tlb_def state.defs)
+
+lemma tlb_incon_more' [simp]:
+  "state.more (typ_incon' s) = tlb_incon_set' s"
+  by (clarsimp simp: typ_incon'_def state.defs)
+
+lemma tlb_truncate [simp]:
+  "state.truncate (typ_tlb s') = state.truncate s'"
+  by (clarsimp simp: typ_tlb_def state.defs)
+
+lemma tlb_det_truncate [simp]:
+  "state.truncate (typ_det_tlb s') = state.truncate s'"
+  by (clarsimp simp: typ_det_tlb_def state.defs)
+
+lemma tlb_sat_no_flt_truncate [simp]:
+  "state.truncate (typ_sat_no_flt_tlb s') = state.truncate s'"
+  by (clarsimp simp: typ_sat_no_flt_tlb_def state.defs)
+
+lemma tlb_incon_truncate' [simp]:
+  "state.truncate (typ_incon' s') = state.truncate s'"
+  by (clarsimp simp: typ_incon'_def state.defs)
+
+
+lemma typ_prim_parameter [simp]:
+  "ASID (typ_tlb s) = ASID s \<and> TTBR0 (typ_tlb s) =  TTBR0 s \<and> MEM (typ_tlb s) = MEM s \<and>
+      exception (typ_tlb s) = exception s"
+  by (clarsimp simp: typ_tlb_def  state.defs)
+
+
+lemma typ_det_prim_parameter [simp]:
+  "ASID (typ_det_tlb s) = ASID s \<and> TTBR0 (typ_det_tlb s) =  TTBR0 s \<and> MEM (typ_det_tlb s) = MEM s \<and>
+      exception (typ_det_tlb s) = exception s"
+  by (clarsimp simp: typ_det_tlb_def state.defs)
+
+
+lemma typ_sat_no_flt_prim_parameter [simp]:
+  "ASID (typ_sat_no_flt_tlb s) = ASID s \<and> TTBR0 (typ_sat_no_flt_tlb s) =  TTBR0 s \<and> MEM (typ_sat_no_flt_tlb s) = MEM s \<and>
+      exception (typ_sat_no_flt_tlb s) = exception s"
+  by (clarsimp simp: typ_sat_no_flt_tlb_def state.defs)
+
+
+lemma typ_incon_prim_parameter' [simp]:
+  "ASID (typ_incon' s) = ASID s \<and> TTBR0 (typ_incon' s) =  TTBR0 s \<and> MEM (typ_incon' s) = MEM s \<and>
+      exception (typ_incon' s) = exception s"
+  by (clarsimp simp: typ_incon'_def state.defs)
+
+
+definition
+  "consistent0 m asid ttbr0 tlb va \<equiv>
+     lookup tlb asid (addr_val va) = Hit (pt_walk asid m ttbr0 va) \<or>
+     lookup tlb asid (addr_val va) = Miss"
+
+
+abbreviation
+  "consistent (s::tlb_entry set state_scheme) \<equiv>
+               consistent0 (MEM s) (ASID s) (TTBR0 s) (state.more s)"
+
+(* TLB doesn't store page faults in this level of the model *)
+definition
+  "no_faults tlb = (\<forall>e \<in> tlb. \<not>is_fault e)"
+
+
+definition 
+   asid_va_incon :: "tlb \<Rightarrow> (asid \<times> vaddr) set"
+where                                                         
+  "asid_va_incon tlb  \<equiv>  {(asid, va). lookup tlb asid (addr_val va) = Incon}"
+
+
+definition
+  saturated_no_flt :: "tlb_entry set state_scheme \<Rightarrow> bool"
+where
+  "saturated_no_flt s  \<equiv> {e\<in>pt_walk (ASID s) (MEM s) (TTBR0 s) ` UNIV. \<not> is_fault e} \<subseteq> state.more s"
+
+
+definition
+  tlb_rel :: "tlb_entry set state_scheme \<Rightarrow> tlb_entry set state_scheme \<Rightarrow> bool"
+where
+  "tlb_rel s t \<equiv> state.truncate s = state.truncate t \<and> state.more s \<subseteq> state.more t  \<and> no_faults (state.more t)"
+
+
+definition 
+  tlb_rel_sat_no_flt :: "tlb_entry set state_scheme \<Rightarrow> tlb_entry set state_scheme \<Rightarrow> bool"
+where                                                                
+  "tlb_rel_sat_no_flt s t \<equiv> state.truncate s = state.truncate t \<and> state.more s \<subseteq> state.more t \<and> saturated_no_flt t \<and> no_faults (state.more t)"
+
+
+
+
+(* for current state's asid and root only *)
+
+definition                              
+   asid_va_hit_incon :: "tlb_entry set state_scheme \<Rightarrow> (asid \<times> vaddr) set"
+where                                                         
+  "asid_va_hit_incon s  \<equiv>  {(asid, va). asid = ASID s \<and>  
+                            (\<exists>x. lookup (state.more s) asid (addr_val va) = Hit x \<and> x \<noteq> pt_walk (ASID s) (MEM s) (TTBR0 s) va ) }"
+
+(*  should we here reload for all the assigned asid? ,
+    might be not, as we are reloading only for the current asid later *)       
+
+definition                              
+   asid_va_incon_tlb_mem :: "tlb_entry set state_scheme \<Rightarrow> (asid \<times> vaddr) set"
+where                                                         
+  "asid_va_incon_tlb_mem s  \<equiv>  asid_va_incon (state.more s) \<union> asid_va_hit_incon s "
+
+
+
+definition 
+  snapshot_of_tlb :: "tlb \<Rightarrow>  asid \<Rightarrow> vaddr \<Rightarrow> lookup_type"
+where                                                                
+  "snapshot_of_tlb t \<equiv> (\<lambda> a v. lookup t a (addr_val v))"
+
+
+definition 
+  tlb_rel_abs' :: "tlb_entry set state_scheme \<Rightarrow> tlb_incon_set' state_scheme \<Rightarrow> bool"
+where                                                                
+  "tlb_rel_abs' s t \<equiv> state.truncate s = state.truncate t \<and>  asid_va_incon_tlb_mem s \<subseteq> incon_set (state.more t) \<and> 
+                       saturated_no_flt s \<and> no_faults (state.more s) \<and> 
+                         (\<forall>a v. a \<noteq> ASID s \<longrightarrow> snapshot_of_tlb (state.more s) a v \<le> tlb_snapshot (state.more t) a  v) \<and>
+                          {(a,v). tlb_snapshot (state.more t) a  v = Incon }  \<subseteq>  incon_set (state.more t)" 
+
+
+(* have proved the update ASID with the equality version of last conj, but for write we need the subset relation *)
+
+(* should we add a condition that all of the elements in the incon set has incon in the saturated tlb, not the 
+  hit or a miss? or its not necessary, why it is not necessary? *)
+
+
+consts tlb_evict :: "tlb_entry set state_scheme \<Rightarrow> tlb_entry set"
+
+
+declare return_def [simp add]
+declare bind_def [simp add]
+declare read_state_def [simp add]
+declare update_state_def [simp add]
+declare extend_state_def [simp add]
+declare trim_state_def [simp add]
+
+
+
+
+lemma consistent_not_Incon:
+  "consistent0 m asid ttbr0 tlb va = 
+  (lookup tlb asid (addr_val va) \<noteq> Incon \<and> (\<forall>e. lookup tlb asid (addr_val va) = Hit e \<longrightarrow> e = pt_walk asid m ttbr0 va))"
+  by (cases "lookup tlb asid (addr_val va)"; simp add: consistent0_def)
+
+
+lemma tlb_relD:
+  "tlb_rel s t \<Longrightarrow> ASID t = ASID s \<and> MEM t = MEM s \<and> TTBR0 t = TTBR0 s \<and>
+      state.more s \<subseteq> state.more t \<and> exception t = exception s"
+  by (clarsimp simp: tlb_rel_def state.defs)
+
+lemma tlb_rel_consistent:
+  "\<lbrakk> tlb_rel s t; consistent t va \<rbrakk> \<Longrightarrow> 
+          consistent s va"
+  apply (drule tlb_relD)
+  apply clarsimp
+  apply (drule tlb_mono [of _ _ "ASID s" "(addr_val va)"])
+  by (auto simp: consistent0_def less_eq_lookup_type typ_det_tlb_def state.defs)
+
+
+
+lemma tlb_rel_no_flt_satD:
+  "tlb_rel_sat_no_flt s t \<Longrightarrow>
+      ASID t = ASID s \<and> MEM t = MEM s \<and> TTBR0 t = TTBR0 s \<and>  state.more s \<subseteq>  state.more t \<and> exception t = exception s"
+  by (clarsimp simp: tlb_rel_sat_no_flt_def state.defs)
+
+
+lemma tlb_rel_sat_no_flt_consistent:
+  "\<lbrakk> tlb_rel_sat_no_flt s t; consistent t va \<rbrakk> \<Longrightarrow> consistent s va"
+  apply (drule  tlb_rel_no_flt_satD)
+  apply clarsimp
+  apply (drule tlb_mono [of _ _ "ASID s" "(addr_val va)"])
+  apply (auto simp: consistent0_def less_eq_lookup_type)
+  done
+
+
+(*find_theorems consistent
+  thm consistent_tlb_state_ext_def
+  help*)
+
+lemma lookup_in_tlb:
+  "lookup tlb asid va = Hit e \<Longrightarrow> e \<in> tlb"
+  by (auto simp: lookup_def entry_set_def split: if_split_asm)
+
+lemma entry_set_insert:
+  "\<lbrakk> entry_set tlb asid va = {}; asid_entry e = asid; va \<in> entry_range e \<rbrakk> \<Longrightarrow> 
+  entry_set (insert e tlb) asid va = {e}"
+  by (auto simp add: entry_set_def entry_range_asid_tags_def)
+
+lemma asid_entry_pt_walk [simp]:
+  "asid_entry (pt_walk asid m ttbr0 va) = asid"
+  apply (simp add: pt_walk_def Let_def)
+  apply ((((cases "get_pde m ttbr0 va" ; clarsimp) , case_tac a ; clarsimp) , 
+      case_tac "get_pte m x3 va" ; clarsimp) , case_tac a ; clarsimp)
+  done
+
+lemma va_20_left [simp]:
+  fixes va :: "32 word"
+  shows "ucast (ucast (va >> 20) :: 12 word) << 20 \<le> va"
+  by word_bitwise
+
+lemma va_12_left [simp]:
+  fixes va :: "32 word"
+  shows "ucast (ucast (va >> 12) :: 20 word) << 12 \<le> va"
+  by word_bitwise
+
+lemma va_20_right [simp]:
+  fixes va :: "32 word"
+  shows "va \<le> (ucast (ucast (va >> 20) :: 12 word) << 20) + 0x000FFFFF"
+  by word_bitwise
+
+lemma va_12_right [simp]:
+  fixes va :: "32 word"
+  shows "va \<le> (ucast (ucast (va >> 12) :: 20 word) << 12) + 0x00000FFF"
+  by word_bitwise
+
+lemma asid_entry_range [simp, intro!]:
+  "addr_val va \<in> entry_range (pt_walk asid m ttbr0 va)"
+  apply (clarsimp simp: entry_range_def pt_walk_def Let_def)
+  by ((((cases "get_pde m ttbr0 va" ; clarsimp) , case_tac a ; clarsimp) , 
+      case_tac "get_pte m x3 va" ; clarsimp) , case_tac a ; clarsimp)
+
+lemma asid_entry_range1 [simp, intro!]:
+  "va \<in> entry_range (pt_walk asid m ttbr0 (Addr va))"
+  apply (clarsimp simp: entry_range_def pt_walk_def Let_def)
+  by ((((cases "get_pde m ttbr0 (Addr va)" ; clarsimp) , case_tac a ; clarsimp) , 
+      case_tac "get_pte m x3 (Addr va)" ; clarsimp) , case_tac a ; clarsimp)
+
+
+lemma lookup_refill:
+  "lookup tlb asid (addr_val va) = Miss \<Longrightarrow>
+   lookup (insert (pt_walk asid m ttbr va) tlb) asid (addr_val va) = Hit (pt_walk asid m ttbr va)"
+   by (clarsimp simp: lookup_def entry_set_insert [where e="pt_walk asid m ttbr va"] split: if_split_asm)
+
+
+lemma consistent_insert [simp, intro!]:
+  "lookup tlb asid (addr_val va) = Miss \<Longrightarrow>
+  consistent0 m asid ttbr (insert (pt_walk asid m ttbr va) tlb) va"
+  by (simp add: consistent0_def lookup_refill)
+
+
+
+(******************************)
+
+
+lemma lookup_incon_subset [simp]:
+  "\<lbrakk> s \<subseteq> t ; lookup s a va = Incon \<rbrakk> \<Longrightarrow> 
+       lookup t a va = Incon"
+  by (metis less_eq_lookup_type lookup_type.simps(3) tlb_mono)
+
+
+lemma  lookup_saturated_no_flt_miss_is_fault:
+  "lookup (tlb_sat_no_flt_set s \<union> {e \<in> range (pt_walk (ASID s) (MEM s) (TTBR0 s)). \<not> is_fault e}) (ASID s) (addr_val va) = Miss \<Longrightarrow>
+    is_fault (pt_walk (ASID s) (MEM s) (TTBR0 s) va)  "
+  apply (clarsimp simp: lookup_def entry_set_def entry_range_asid_tags_def split: if_split_asm)
+  by force
+
+
+lemma 
+  "\<lbrakk>lookup (t1 \<union> t2) a va = Hit x ; t2 \<subseteq> t1 \<rbrakk>  \<Longrightarrow>  entry_set t1 a va = {x} "
+  apply (clarsimp simp: lookup_def split:if_split_asm)
+  apply (clarsimp simp: entry_set_def)
+  by auto 
+
+
+
+lemma
+  "\<lbrakk>consistent (typ_sat_no_flt_tlb s) va ; 
+    lookup (tlb_sat_no_flt_set s) (ASID s) (addr_val va) = Hit x3 \<rbrakk> \<Longrightarrow>  x3 = pt_walk (ASID s) (MEM s) (TTBR0 s) va"
+  apply (clarsimp simp: consistent0_def )
+done
+
+
+
+
+(* IMPORTANT *)
+
+
+lemma write'mem1_eq_TLB:
+  "\<lbrakk> write'mem1 (val, va, sz) s = ((), s') \<rbrakk>  \<Longrightarrow> state.more s' = state.more s"
+   by (clarsimp simp: write'mem1_def raise'exception_def split: if_split_asm)
+
+
+lemma write_same_mem:
+  "\<lbrakk> write'mem1 (val, va, sz) s = ((), s') ; write'mem1 (val, va, sz) t = ((), t') ;
+      MEM s = MEM t\<rbrakk>  \<Longrightarrow>  MEM s' = MEM t'"
+  by (clarsimp simp: write'mem1_def raise'exception_def split:if_split_asm)
+
+lemma write_same_mem_excep:
+  "\<lbrakk> write'mem1 (val, pa, sz) s = ((), s') ; write'mem1 (val, pa, sz) t = ((), t') ;
+      MEM s = MEM t ; exception s = exception t \<rbrakk>  \<Longrightarrow> exception s' = exception t'"
+   apply (clarsimp simp: write'mem1_def raise'exception_def split:if_split_asm)
+done
+
+ 
+
+lemma write'mem1_rel:
+  "\<lbrakk> write'mem1 (val, va, sz) s = ((), s') \<rbrakk>  \<Longrightarrow> s' = s \<lparr> MEM:= MEM s' , exception:= exception s' \<rparr>"
+   by (clarsimp simp: write'mem1_def raise'exception_def split: if_split_asm)
+
+
+
+lemma sat_state_tlb':
+  "\<lbrakk> saturated_no_flt s \<rbrakk> \<Longrightarrow> 
+     state.more s = state.more s \<union> {e\<in>pt_walk (ASID s) (MEM s) (TTBR0 s) ` UNIV. \<not> is_fault e}"
+  by (fastforce simp: saturated_no_flt_def)
+
+
+lemma tlb_rel'_absD:
+  "tlb_rel_abs' s t \<Longrightarrow>
+     ASID t = ASID s \<and> MEM t = MEM s \<and> TTBR0 t = TTBR0 s \<and>  saturated_no_flt s \<and> no_faults (state.more s)
+         \<and> asid_va_incon_tlb_mem s  \<subseteq> incon_set (state.more t) \<and> exception t = exception s"
+   by (clarsimp simp: tlb_rel_abs'_def state.defs)
+
+
+end
