MMU_ARMv7_Refinement_No_Fault/ARMv7_Update_ASID_Ref.thy
@@ -1,0 +1,485 @@
+theory ARMv7_Update_ASID_Ref
+
+
+imports  ARMv7_Update_TTBR0_Ref
+
+begin  
+
+
+
+class update_asid =
+  fixes update_asid :: "asid \<Rightarrow> 'a state_scheme \<Rightarrow>  unit \<times> 'a state_scheme" 
+
+
+instantiation tlb_state_ext :: (type) update_asid   
+begin
+  definition   
+  "(update_asid a :: ('a tlb_state_scheme \<Rightarrow> _))  = update_state (\<lambda>s. s\<lparr> ASID := a \<rparr>) "
+
+thm update_asid_tlb_state_ext_def
+(* print_context *)                      
+  instance ..
+end
+
+
+instantiation tlb_det_state_ext :: (type) update_asid   
+begin
+  definition   
+  "(update_asid a :: ('a tlb_det_state_scheme \<Rightarrow> _))  = update_state (\<lambda>s. s\<lparr> ASID := a \<rparr>) "
+
+thm update_asid_tlb_det_state_ext_def
+(* print_context *)                      
+  instance ..
+end
+
+
+
+
+
+instantiation tlb_sat_no_flt_state_ext :: (type) update_asid   
+begin
+  definition   
+  "(update_asid a :: ('a tlb_sat_no_flt_state_scheme \<Rightarrow> _))  = do {
+      update_state (\<lambda>s. s\<lparr> ASID := a \<rparr>);
+      mem   <- read_state MEM;
+      ttbr0 <- read_state TTBR0;
+      let all_non_fault_entries = {e\<in>pt_walk a mem ttbr0 ` UNIV. \<not>is_fault e};
+      tlb0   <- read_state tlb_sat_no_flt_set;
+      let tlb = tlb0 \<union> all_non_fault_entries; 
+      update_state (\<lambda>s. s\<lparr> tlb_sat_no_flt_set := tlb \<rparr>)} "
+
+thm update_asid_tlb_sat_no_flt_state_ext_def
+(* print_context *)                      
+  instance ..
+end
+
+
+definition 
+  incon_load :: "(asid \<Rightarrow> vaddr \<Rightarrow> lookup_type) \<Rightarrow> asid \<Rightarrow> heap \<Rightarrow> ttbr0 \<Rightarrow> (asid \<times> vaddr) set"
+  where
+  "incon_load snp a m rt \<equiv> (\<lambda>v. (a, v) ) ` 
+                            {v. \<exists>x. snp a v = Hit x \<and> x \<noteq> pt_walk a m rt v}"
+
+definition 
+  miss_to_hit :: "(asid \<Rightarrow> vaddr \<Rightarrow> lookup_type) \<Rightarrow> asid \<Rightarrow> heap \<Rightarrow> ttbr0 \<Rightarrow> (asid \<times> vaddr) set"
+ where
+  "miss_to_hit snp a m rt \<equiv> (\<lambda>v. (a, v) ) ` 
+                              {v. snp a v = Miss \<and>  \<not>is_fault (pt_walk a m rt v)}"
+
+definition 
+  consistent_hit :: "(asid \<Rightarrow> vaddr \<Rightarrow> lookup_type) \<Rightarrow> asid \<Rightarrow> heap \<Rightarrow> ttbr0 \<Rightarrow> (asid \<times> vaddr) set"
+ where
+  "consistent_hit snp a m rt \<equiv> (\<lambda>v. (a, v) ) ` 
+                                 {v. snp a v = Hit (pt_walk a m rt v)}"
+
+
+
+definition 
+  snapshot_update_new :: "(asid \<times> vaddr) set \<Rightarrow> (asid \<times> vaddr) set \<Rightarrow> (asid \<times> vaddr) set \<Rightarrow> 
+                          heap \<Rightarrow> ttbr0 \<Rightarrow>  (asid \<Rightarrow> vaddr \<Rightarrow> lookup_type)"
+where
+  "snapshot_update_new iset m_to_h h_to_h hp ttbr0 \<equiv> (\<lambda>x y. if (x,y) \<in>  iset then Incon 
+                                                     else if (x,y) \<in> m_to_h then Hit (pt_walk x hp ttbr0 y) 
+                                                     else if (x,y) \<in> h_to_h then Hit (pt_walk x hp ttbr0 y) 
+                                                     else Miss)"
+
+definition 
+  snapshot_update_new' :: "(asid \<Rightarrow> vaddr \<Rightarrow> lookup_type)  \<Rightarrow> (asid \<times> vaddr) set \<Rightarrow> (asid \<times> vaddr) set \<Rightarrow> (asid \<times> vaddr) set \<Rightarrow> 
+                          heap \<Rightarrow> ttbr0 \<Rightarrow> asid \<Rightarrow> (asid \<Rightarrow> vaddr \<Rightarrow> lookup_type)"
+where
+  "snapshot_update_new' snp iset m_to_h h_to_h hp ttbr0 a \<equiv> 
+                     snp (a := snapshot_update_new iset m_to_h h_to_h hp ttbr0 a)"
+
+(*
+definition 
+  snapshot_update :: "(asid \<times> vaddr) set \<Rightarrow> (asid \<Rightarrow> vaddr \<Rightarrow> lookup_type)"
+where
+  "snapshot_update iset  \<equiv> (\<lambda>x y. if (x,y) \<in>  iset then Incon   else Miss)"
+*)
+
+definition 
+  snapshot_update_current :: "(asid \<times> vaddr) set \<Rightarrow> heap \<Rightarrow> ttbr0 \<Rightarrow>(asid \<Rightarrow> vaddr \<Rightarrow> lookup_type)"
+where
+  "snapshot_update_current iset mem ttbr0  \<equiv> (\<lambda>x y. if (x,y) \<in>  iset then Incon else 
+                            if (\<not>is_fault (pt_walk x mem ttbr0 y)) then  Hit (pt_walk x mem ttbr0 y) else Miss)"
+
+
+
+definition 
+  snapshot_update_current' :: "(asid \<Rightarrow> vaddr \<Rightarrow> lookup_type) \<Rightarrow> (asid \<times> vaddr) set \<Rightarrow> 
+                      heap \<Rightarrow> ttbr0 \<Rightarrow> asid \<Rightarrow> (asid \<Rightarrow> vaddr \<Rightarrow> lookup_type)"
+where
+  "snapshot_update_current' snp iset mem ttbr0 a \<equiv> snp (a := snapshot_update_current iset mem ttbr0 a)"
+
+
+instantiation tlb_incon_state'_ext :: (type) update_asid   
+begin
+  definition   
+  "(update_asid a :: ('a tlb_incon_state'_scheme \<Rightarrow> _))  = do {
+      mem   <- read_state MEM;
+      ttbr0 <- read_state TTBR0;
+      asid  <- read_state ASID;
+      tlb_incon_set   <- read_state tlb_incon_set';
+      let iset = incon_set tlb_incon_set;  
+      let snapshot = tlb_snapshot tlb_incon_set;
+      let iset_current = ({asid} \<times> UNIV) \<inter> iset; 
+      let snapshot_current = snapshot_update_current' snapshot iset_current mem ttbr0 asid;
+      let tlb_incon_set = tlb_incon_set \<lparr>tlb_snapshot := snapshot_current \<rparr>;
+      update_state (\<lambda>s. s\<lparr>tlb_incon_set' := tlb_incon_set \<rparr>);
+
+      (* new ASID *)
+      update_state (\<lambda>s. s\<lparr> ASID := a \<rparr>);
+      
+     let iset_snp = incon_load snapshot_current a mem ttbr0; 
+     let iset_new = ({a} \<times> UNIV) \<inter> iset; 
+     let iset_new_snp = iset_new \<union> iset_snp;
+     let m_to_h = miss_to_hit  snapshot_current a mem ttbr0;
+     let h_to_h = consistent_hit snapshot_current a mem ttbr0;
+     let snapshot' = snapshot_update_new' snapshot_current iset_new_snp m_to_h h_to_h mem ttbr0 a;
+     let tlb_incon_set = tlb_incon_set\<lparr> incon_set:= iset \<union> iset_snp , tlb_snapshot := snapshot'  \<rparr>;
+     update_state (\<lambda>s. s\<lparr> tlb_incon_set' := tlb_incon_set \<rparr>)
+} "
+thm update_asid_tlb_incon_state'_ext_def
+print_context                     
+  instance ..
+end
+
+
+
+
+lemma update_asid_non_det_det_refine:
+  "\<lbrakk> update_asid a (s::tlb_state) = ((), s') ;  update_asid a (t::tlb_det_state) = ((), t'); 
+         tlb_rel (typ_tlb s) (typ_det_tlb t) \<rbrakk> \<Longrightarrow>  tlb_rel (typ_tlb s') (typ_det_tlb t') "
+  apply (clarsimp simp: update_asid_tlb_state_ext_def update_asid_tlb_det_state_ext_def tlb_rel_def) 
+  by (cases s, cases t , clarsimp simp: state.defs)
+
+
+lemma  update_asid_det_sat_no_flt_refine:
+  "\<lbrakk> update_asid a (s::tlb_det_state) = ((), s') ;  update_asid a (t::tlb_sat_no_flt_state) = ((), t'); 
+         tlb_rel_sat_no_flt (typ_det_tlb s) (typ_sat_no_flt_tlb t) \<rbrakk> \<Longrightarrow> 
+                  tlb_rel_sat_no_flt (typ_det_tlb s') (typ_sat_no_flt_tlb t')"
+  apply (clarsimp simp: update_asid_tlb_det_state_ext_def update_asid_tlb_sat_no_flt_state_ext_def)
+  apply (clarsimp simp: tlb_rel_sat_no_flt_def saturated_no_flt_def no_faults_def)
+  apply (cases s, cases t , clarsimp simp: state.defs , force)
+done
+
+lemma  lookup_incon_not_miss:
+   "\<lbrakk> lookup (t \<union> t') a v = Incon ; lookup t' a v = Miss\<rbrakk> \<Longrightarrow>
+       lookup t a v = Incon"
+  apply (clarsimp simp: lookup_def entry_set_def split: if_split_asm)
+  apply safe
+  by force+
+
+lemma lookup_hit_diff_union_incon:
+  "\<lbrakk>lookup t a v = Hit x ; lookup t' a v = Hit x' ; x \<noteq> x'\<rbrakk> \<Longrightarrow> lookup (t \<union> t') a v = Incon"
+  apply (clarsimp simp: lookup_def entry_set_def entry_range_asid_tags_def split: if_split_asm)
+  apply safe
+     apply force
+    apply (metis (no_types, lifting) mem_Collect_eq singletonD singletonI)
+   apply (metis (no_types, lifting) mem_Collect_eq singletonD singletonI)
+  apply force
+  done
+
+
+lemma asid_va_incon_rewrite:
+  "\<lbrakk> a \<noteq> ASID s\<rbrakk> \<Longrightarrow> 
+   asid_va_incon (tlb_sat_no_flt_set s \<union> {e \<in> range (pt_walk a (MEM s) (TTBR0 s)). \<not> is_fault e}) =
+     asid_va_incon (tlb_sat_no_flt_set s) \<union> 
+            ((\<lambda>v. (a, v) ) ` {v. \<exists>x. lookup (tlb_sat_no_flt_set s) a (addr_val v) = Hit x \<and>
+                                       x \<noteq> pt_walk a (MEM s) (TTBR0 s) v \<and> \<not> is_fault (pt_walk a (MEM s) (TTBR0 s) v)})"
+  apply (clarsimp simp: asid_va_incon_def)
+  apply safe
+    apply (case_tac "aa \<noteq> a")
+     apply (drule union_incon_cases1)
+     apply( clarsimp simp: lookup_no_flt_range_pt_walk_not_incon' asid_unequal_miss'')
+    apply clarsimp
+    apply (drule union_incon_cases1)
+    apply (erule disjE)
+     apply( clarsimp simp :lookup_no_flt_range_pt_walk_not_incon')
+    apply (erule disjE)
+     apply clarsimp
+     apply (subgoal_tac "pt_walk a (MEM s) (TTBR0 s) xb = pt_walk a (MEM s) (TTBR0 s) (Addr (addr_val b))")
+      apply clarsimp
+     apply (rule va_entry_set_pt_palk_same)
+     apply (clarsimp simp: lookup_def entry_set_hit_entry_range split: if_split_asm)
+    apply (clarsimp simp :lookup_no_flt_range_pt_walk_not_incon')
+    apply (erule disjE)
+     apply (clarsimp simp :lookup_no_flt_range_pt_walk_not_incon')
+    apply (clarsimp simp:)
+   apply (subgoal_tac "tlb_sat_no_flt_set s \<subseteq> tlb_sat_no_flt_set s \<union> {e \<in> range (pt_walk a (MEM s) (TTBR0 s)). \<not> is_fault e}")
+    apply (drule_tac a = aa and v = "addr_val b" in tlb_mono)
+    apply force
+   apply blast
+  apply (subgoal_tac "lookup {e \<in> range (pt_walk a (MEM s) (TTBR0 s)). \<not> is_fault e} a (addr_val x) = Hit (pt_walk a (MEM s) (TTBR0 s) x)")
+   apply (clarsimp simp: lookup_hit_diff_union_incon)
+  using lookup_range_pt_walk_hit_no_flt apply force
+  done
+
+
+
+lemma tlb_snapshot_rewrite:
+  "(a, b) \<notin> Pair a ` {v. \<exists>x. tlb_snapshot (tlb_incon_set' t) a v = Hit x \<and> x \<noteq> pt_walk a (MEM s) (TTBR0 s) v} \<Longrightarrow>
+     (a, b) \<in> Pair a ` {v.  tlb_snapshot (tlb_incon_set' t) a v = Miss} \<or> 
+       (a, b) \<in> Pair a ` {v.  tlb_snapshot (tlb_incon_set' t) a v = Incon} \<or> 
+         (a, b) \<in> Pair a ` {v. \<exists>x. tlb_snapshot (tlb_incon_set' t) a v = Hit x \<and> x = pt_walk a (MEM s) (TTBR0 s) v}"
+  apply (clarsimp simp: image_iff)
+  using lookup_type.exhaust by auto
+
+lemma tlb_snapshot_rewrite':
+  "(a, v) \<notin> Pair a ` {v. tlb_snapshot (tlb_incon_set' t) a v = Miss \<and> \<not> is_fault (pt_walk a (MEM s) (TTBR0 s) v)} \<Longrightarrow>
+       tlb_snapshot (tlb_incon_set' t) a v \<noteq> Miss \<or> (tlb_snapshot (tlb_incon_set' t) a v = Miss \<and> is_fault (pt_walk a (MEM s) (TTBR0 s) v))"
+  by (clarsimp simp: image_iff)
+
+lemma lookup_miss_union_hit_intro:
+  "\<lbrakk>lookup t a v = Miss;  lookup t' a v = Hit x\<rbrakk> \<Longrightarrow> 
+           lookup (t \<union> t') a v = Hit x"
+  apply (clarsimp simp: lookup_def entry_set_def entry_range_asid_tags_def split: if_split_asm)
+  apply safe
+       apply auto 
+  by force
+
+
+lemma lookup_miss_union_hit_intro':
+  "\<lbrakk> lookup t a v = Hit x ; lookup t' a v = Miss\<rbrakk> \<Longrightarrow> 
+           lookup (t \<union> t') a v = Hit x"
+  apply (clarsimp simp: lookup_def entry_set_def entry_range_asid_tags_def split: if_split_asm)
+  apply safe
+       apply auto 
+  by blast
+
+
+lemma lookup_union_hit_hit:
+  "\<lbrakk> lookup t a v = Hit x ; lookup t' a v = Hit x\<rbrakk> \<Longrightarrow> 
+           lookup (t \<union> t') a v = Hit x"
+  apply (clarsimp simp: lookup_def entry_set_def entry_range_asid_tags_def split: if_split_asm)
+  apply safe
+       apply auto 
+  by blast+
+
+
+lemma
+  "\<lbrakk> lookup t a v \<noteq> Incon; lookup t a v \<noteq> Miss\<rbrakk>
+         \<Longrightarrow> \<exists>x\<in>t. lookup t a v = Hit x"
+  apply (clarsimp simp: lookup_def entry_set_def split: if_split_asm) 
+  by blast
+
+
+
+lemma not_miss_incon_hit':
+  " lookup t a va = Incon \<or> (\<exists>x\<in>t. lookup t a va = Hit x) \<Longrightarrow> lookup t a va \<noteq> Miss "
+ by (clarsimp simp: lookup_def entry_set_def split: if_split_asm)
+ 
+
+
+lemma not_fault_range_not_miss:
+  "\<not> is_fault (pt_walk (ASID s) (MEM s) (TTBR0 s) v) \<Longrightarrow> lookup (tlb_sat_no_flt_set s \<union> {e \<in> range (pt_walk (ASID s) (MEM s) (TTBR0 s)). \<not> is_fault e}) (ASID s) (addr_val v) \<noteq> Miss"
+  apply (clarsimp simp:)
+  apply (clarsimp simp: lookup_def entry_set_va_set  a_va_set_def split: if_split_asm)
+  apply (drule_tac x = "pt_walk (ASID s) (MEM s) (TTBR0 s) v" in bspec)
+   apply (drule_tac x = "pt_walk (ASID s) (MEM s) (TTBR0 s) v" in spec)
+   apply clarsimp
+   apply (insert asid_va_entry_range_pt_entry [of "ASID s" "addr_val v" "MEM s" "TTBR0 s" ] , clarsimp)
+  apply clarsimp
+  done
+
+
+
+lemma update_asid_sat_no_flt_abs_refine':
+  "\<lbrakk> update_asid a (s::tlb_sat_no_flt_state) = ((), s') ;  update_asid a (t::tlb_incon_state') = ((), t'); 
+        tlb_rel_abs' (typ_sat_no_flt_tlb s) (typ_incon' t) \<rbrakk> \<Longrightarrow> 
+                       tlb_rel_abs' (typ_sat_no_flt_tlb s') (typ_incon' t')"
+  apply (clarsimp simp: update_asid_tlb_sat_no_flt_state_ext_def update_asid_tlb_incon_state'_ext_def Let_def)
+  apply (frule tlb_rel'_absD)
+  apply (case_tac "a = ASID s")
+    (* when we update to the same ASID *)
+   apply (subgoal_tac "tlb_sat_no_flt_set s = tlb_sat_no_flt_set s \<union> 
+         {e \<in> range (pt_walk (ASID s) (MEM s) (TTBR0 s)). \<not> is_fault e}")
+    prefer 2
+    apply (clarsimp simp:  saturated_no_flt_def) 
+    apply blast
+   apply clarsimp
+   apply (clarsimp simp: tlb_rel_abs'_def)
+   apply (rule conjI)
+    apply (clarsimp simp: state.defs)
+   apply (rule conjI)
+    apply force
+   apply (rule conjI)
+    apply clarsimp
+    apply (clarsimp simp: snapshot_of_tlb_def snapshot_update_current'_def snapshot_update_current_def
+                        snapshot_update_new'_def  snapshot_update_new_def)
+   apply (clarsimp simp: snapshot_of_tlb_def snapshot_update_current'_def snapshot_update_current_def
+                        snapshot_update_new'_def  snapshot_update_new_def incon_load_def)
+   apply force
+
+
+
+(* when we update to the new ASID *)
+  apply (clarsimp simp: tlb_rel_abs'_def)
+  apply (rule conjI)
+   apply (clarsimp simp: state.defs)
+  apply (rule conjI)
+   apply (clarsimp simp: asid_va_incon_tlb_mem_def)
+   apply (rule conjI)
+    apply (subgoal_tac "asid_va_incon (tlb_sat_no_flt_set s \<union> {e \<in> range (pt_walk a (MEM s) (TTBR0 s)). \<not> is_fault e}) =
+     asid_va_incon (tlb_sat_no_flt_set s) \<union> 
+            ((\<lambda>v. (a, v) ) ` {v. \<exists>x. lookup (tlb_sat_no_flt_set s) a (addr_val v) = Hit x \<and>
+                                       x \<noteq> pt_walk a (MEM s) (TTBR0 s) v \<and> \<not> is_fault (pt_walk a (MEM s) (TTBR0 s) v)})")
+     prefer 2
+     apply (clarsimp simp: asid_va_incon_rewrite)
+    apply (simp only:)
+    apply (thin_tac "asid_va_incon (tlb_sat_no_flt_set s \<union> {e \<in> range (pt_walk a (MEM s) (TTBR0 s)). \<not> is_fault e}) =
+     asid_va_incon (tlb_sat_no_flt_set s) \<union>
+     Pair a `
+     {v. \<exists>x. lookup (tlb_sat_no_flt_set s) a (addr_val v) = Hit x \<and> x \<noteq> pt_walk a (MEM s) (TTBR0 s) v \<and> \<not> is_fault (pt_walk a (MEM s) (TTBR0 s) v)}")
+    apply (simp only: incon_load_def snapshot_update_current'_def snapshot_update_current_def)
+    apply (subgoal_tac " Pair a `
+        {v. \<exists>x. lookup (tlb_sat_no_flt_set s) a (addr_val v) = Hit x \<and> x \<noteq> pt_walk a (MEM s) (TTBR0 s) v \<and> \<not> is_fault (pt_walk a (MEM s) (TTBR0 s) v)}
+        \<subseteq> incon_set (tlb_incon_set' t) \<union>
+           Pair a `
+           {v. \<exists>x. ((tlb_snapshot (tlb_incon_set' t))
+                    (ASID s :=
+                       \<lambda>y. if (ASID s, y) \<in> {ASID s} \<times> UNIV \<inter> incon_set (tlb_incon_set' t) then Incon
+                           else if \<not> is_fault (pt_walk (ASID s) (MEM s) (TTBR0 s) y) then Hit (pt_walk (ASID s) (MEM s) (TTBR0 s) y)
+                                else Miss))
+                    a v =
+                   Hit x \<and>
+                   x \<noteq> pt_walk a (MEM s) (TTBR0 s) v}")
+     apply blast
+    apply rule
+    apply (clarsimp simp: snapshot_of_tlb_def)
+    apply (subgoal_tac " tlb_snapshot (tlb_incon_set' t) a x = Hit xa \<or>  tlb_snapshot (tlb_incon_set' t) a x = Incon")
+     apply (erule disjE)
+      apply force
+     (* last assumption of tlb_rel_abs' is needed here , in the case of update asid, only equality is required*)
+     apply force
+    apply (rule disjCI)
+    apply (force simp: less_eq_lookup_type)
+   apply (clarsimp simp: asid_va_hit_incon_def)
+   apply (clarsimp simp: incon_load_def snapshot_of_tlb_def  snapshot_update_current'_def snapshot_update_current_def)
+   apply (drule tlb_snapshot_rewrite)
+   apply (erule disjE)
+    apply (subgoal_tac "lookup (tlb_sat_no_flt_set s) a (addr_val b) = Miss")
+     prefer 2
+     apply (clarsimp simp: image_iff)
+     apply (drule_tac x = a in spec, clarsimp)
+     apply (drule_tac x = b in spec)
+     apply force
+    apply (drule lookup_hit_union_cases')
+    apply (erule disjE , clarsimp)
+    apply (erule disjE)
+     apply clarsimp
+     apply (frule lookup_range_fault_pt_walk)
+     apply (subgoal_tac "(addr_val xa) \<in> entry_range x")
+      apply force
+     apply (clarsimp simp: lookup_def lookup_hit_entry_range split: if_split_asm)
+    apply clarsimp
+   apply (erule disjE)
+    apply force
+   apply (drule lookup_hit_union_cases')
+   apply (erule disjE)
+    apply clarsimp
+    apply (subgoal_tac " x = pt_walk a (MEM s) (TTBR0 s) xa")
+     apply clarsimp
+    apply (drule_tac x = a in spec, clarsimp)
+    apply (drule_tac x = xa in spec)
+    apply (force simp: less_eq_lookup_type)
+   apply (erule disjE , clarsimp)
+    apply (frule lookup_range_fault_pt_walk)
+    apply (subgoal_tac "(addr_val xa) \<in> entry_range x")
+     apply force
+    apply (clarsimp simp: lookup_def lookup_hit_entry_range split: if_split_asm)
+   apply clarsimp    
+   apply (frule lookup_range_fault_pt_walk)
+   apply (subgoal_tac "(addr_val xa) \<in> entry_range x")
+    apply force
+   apply (clarsimp simp: lookup_def lookup_hit_entry_range split: if_split_asm)
+
+  apply (rule conjI)
+   apply (clarsimp simp: saturated_no_flt_def)
+  apply (rule conjI)
+   apply (clarsimp simp: no_faults_def)
+
+  apply (thin_tac " t' = t\<lparr>ASID := a, tlb_incon_set' := tlb_incon_set' t
+                         \<lparr>incon_set := incon_set (tlb_incon_set' t) \<union> incon_load (snapshot_update_current' (tlb_snapshot (tlb_incon_set' t)) ({ASID s} \<times> UNIV \<inter> incon_set (tlb_incon_set' t)) (MEM s) (TTBR0 s) (ASID s)) a (MEM s) (TTBR0 s),
+                            tlb_snapshot :=
+                              snapshot_update_new' (snapshot_update_current' (tlb_snapshot (tlb_incon_set' t)) ({ASID s} \<times> UNIV \<inter> incon_set (tlb_incon_set' t)) (MEM s) (TTBR0 s) (ASID s))
+                               ({a} \<times> UNIV \<inter> incon_set (tlb_incon_set' t) \<union> incon_load (snapshot_update_current' (tlb_snapshot (tlb_incon_set' t)) ({ASID s} \<times> UNIV \<inter> incon_set (tlb_incon_set' t)) (MEM s) (TTBR0 s) (ASID s)) a (MEM s) (TTBR0 s))
+                               (miss_to_hit (snapshot_update_current' (tlb_snapshot (tlb_incon_set' t)) ({ASID s} \<times> UNIV \<inter> incon_set (tlb_incon_set' t)) (MEM s) (TTBR0 s) (ASID s)) a (MEM s) (TTBR0 s))
+                               (consistent_hit (snapshot_update_current' (tlb_snapshot (tlb_incon_set' t)) ({ASID s} \<times> UNIV \<inter> incon_set (tlb_incon_set' t)) (MEM s) (TTBR0 s) (ASID s)) a (MEM s) (TTBR0 s)) (MEM s) (TTBR0 s) a\<rparr>\<rparr>")
+
+(* relationship between snapshot_of_tlb and tlb_snapshot *)
+
+  apply (rule conjI)
+   apply (rule allI)
+   apply (rule impI)
+   apply (rule allI)
+   apply (case_tac "aa \<noteq> ASID s")
+    apply (simp only: snapshot_of_tlb_def snapshot_update_new'_def snapshot_update_new_def snapshot_update_current'_def snapshot_update_current_def)
+    apply clarsimp
+    apply (subgoal_tac "lookup (tlb_sat_no_flt_set s \<union> {e \<in> range (pt_walk a (MEM s) (TTBR0 s)). \<not> is_fault e}) aa (addr_val v) =
+         lookup (tlb_sat_no_flt_set s) aa (addr_val v)")
+     apply clarsimp
+    apply (rule lookup_miss_union_equal)
+    apply (clarsimp simp: asid_unequal_miss'')
+   apply clarsimp
+   apply (simp only: snapshot_of_tlb_def snapshot_update_new'_def snapshot_update_new_def snapshot_update_current'_def snapshot_update_current_def)
+   apply clarsimp
+   apply (rule conjI)
+    apply clarsimp
+    apply (subgoal_tac "lookup (tlb_sat_no_flt_set s \<union> {e \<in> range (pt_walk a (MEM s) (TTBR0 s)). \<not> is_fault e}) (ASID s) (addr_val v) =
+               lookup (tlb_sat_no_flt_set s) (ASID s) (addr_val v)")
+     prefer 2
+     apply (rule lookup_miss_union_equal)
+     apply (clarsimp simp: asid_unequal_miss'')
+    apply clarsimp
+    apply (subgoal_tac " lookup (tlb_sat_no_flt_set s) (ASID s) (addr_val v) \<noteq> Incon")
+     prefer 2
+     apply (clarsimp simp:  asid_va_incon_tlb_mem_def asid_va_incon_def)
+     apply force
+    apply (subgoal_tac "lookup (tlb_sat_no_flt_set s) (ASID s) (addr_val v) = Miss \<or> lookup (tlb_sat_no_flt_set s) (ASID s) (addr_val v) = Hit (pt_walk (ASID s) (MEM s) (TTBR0 s) v)")
+     apply force
+    apply (rule disjI2)
+    apply (clarsimp simp:  asid_va_incon_tlb_mem_def asid_va_hit_incon_def)
+    apply (subgoal_tac "lookup (tlb_sat_no_flt_set s) (ASID s) (addr_val v) \<noteq> Miss")
+     apply (subgoal_tac "\<exists>x\<in>tlb_sat_no_flt_set s. lookup (tlb_sat_no_flt_set s) (ASID s) (addr_val v) = Hit x")
+      apply force
+     apply (clarsimp simp: lookup_def entry_set_def split: if_split_asm) 
+     apply blast
+    apply (subgoal_tac "lookup (tlb_sat_no_flt_set s \<union> 
+         {e \<in> range (pt_walk (ASID s) (MEM s) (TTBR0 s)). \<not> is_fault e}) (ASID s) (addr_val v) \<noteq> Miss")
+     apply (subgoal_tac "tlb_sat_no_flt_set s = tlb_sat_no_flt_set s \<union> 
+         {e \<in> range (pt_walk (ASID s) (MEM s) (TTBR0 s)). \<not> is_fault e}")
+      prefer 2
+      apply (clarsimp simp:  saturated_no_flt_def) 
+      apply blast
+     apply clarsimp
+    apply (clarsimp simp:  not_fault_range_not_miss)
+   apply clarsimp
+   apply (subgoal_tac "lookup (tlb_sat_no_flt_set s \<union> {e \<in> range (pt_walk a (MEM s) (TTBR0 s)). \<not> is_fault e}) (ASID s) (addr_val v) =
+               lookup (tlb_sat_no_flt_set s) (ASID s) (addr_val v)")
+    prefer 2
+    apply (rule lookup_miss_union_equal)
+    apply (clarsimp simp: asid_unequal_miss'')
+   apply clarsimp
+   apply (subgoal_tac " lookup (tlb_sat_no_flt_set s) (ASID s) (addr_val v) \<noteq> Incon")
+    prefer 2
+    apply (clarsimp simp:  asid_va_incon_tlb_mem_def asid_va_incon_def)
+    apply force
+   apply (subgoal_tac "lookup (tlb_sat_no_flt_set s) (ASID s) (addr_val v) = Miss \<or> 
+                    (\<exists>x\<in>tlb_sat_no_flt_set s. lookup (tlb_sat_no_flt_set s) (ASID s) (addr_val v) = Hit x)")
+    prefer 2
+    apply (clarsimp simp: lookup_def entry_set_def split: if_split_asm) 
+    apply blast
+   apply (erule disjE)
+    apply clarsimp
+   apply clarsimp
+   apply (clarsimp simp:  asid_va_incon_tlb_mem_def asid_va_hit_incon_def)
+   apply (case_tac "x \<noteq> pt_walk (ASID s) (MEM s) (TTBR0 s) v")
+    apply blast
+   apply (clarsimp simp: no_faults_def)
+  apply (clarsimp simp: snapshot_of_tlb_def snapshot_update_new'_def snapshot_update_new_def snapshot_update_current'_def snapshot_update_current_def incon_load_def miss_to_hit_def consistent_hit_def
+      split: if_split_asm)
+  by force
+
+
+end
